block_equiv_checker.v
@@ -150,6 +150,8 @@ Require Import FORVES2.optimizations.strg_solver.
 Import Opt_strg_solver.
 Require Import FORVES2.optimizations.jumpi_neq.
 Import Opt_jumpi_neq.
+Require Import FORVES2.optimizations.lt_ctx.
+Import Opt_lt_ctx.
 
 Require Import FORVES2.symbolic_execution.
 Import SymbolicExecution.
@@ -436,6 +438,7 @@ Inductive available_optimization_step :=
 | OPT_mem_solver
 | OPT_strg_solver
 | OPT_jumpi_neq
+| OPT_lt_ctx
 .
 
 
@@ -511,6 +514,7 @@ match tag with
 | OPT_mem_solver => OpEntry optimize_mem_solver_sbinding optimize_mem_solver_sbinding_snd
 | OPT_strg_solver => OpEntry optimize_strg_solver_sbinding optimize_strg_solver_sbinding_snd
 | OPT_jumpi_neq => OpEntry optimize_jumpi_neq_sbinding optimize_jumpi_neq_sbinding_snd
+| OPT_lt_ctx => OpEntry optimize_lt_ctx_sbinding optimize_lt_ctx_sbinding_snd
 end.
 
 Definition all_optimization_steps := 
@@ -582,6 +586,7 @@ Definition all_optimization_steps :=
    OPT_sgt_x_x
 
    ;OPT_jumpi_neq
+   ;OPT_lt_ctx
    ;OPT_mem_solver
    ;OPT_strg_solver
 ].
@@ -655,6 +660,7 @@ Definition all_optimization_steps' :=
    OPT_sgt_x_x
 
    ;OPT_jumpi_neq
+   ;OPT_lt_ctx
    ;OPT_mem_solver
    ;OPT_strg_solver   
 ].
